transf_initial_states

backend/Duplicateaux.ml
@@ -1,3 +1,4 @@
+open RTL
 open Maps
 
-let duplicate_aux f = (f, PTree.empty)
+let duplicate_aux f = ((fn_code f), PTree.empty)
