backend/Duplicate.v
@@ -6,23 +6,32 @@ Require Import Coqlib Errors.
 
 Local Open Scope error_monad_scope.
 
-(** External oracle returning the new RTL function, along with a mapping
-    of new nodes to old nodes *)
-Axiom duplicate_aux: RTL.function -> RTL.function * (PTree.t nat).
+(** External oracle returning the new RTL code (entry point unchanged),
+    along with a mapping of new nodes to old nodes *)
+Axiom duplicate_aux: RTL.function -> RTL.code * (PTree.t nat).
 
 Extract Constant duplicate_aux => "Duplicateaux.duplicate_aux".
 
 (** * Verification of node duplications *)
 
 (** Verifies that the mapping [mp] is giving correct information *)
-Definition verify_mapping (f tf: function) (mp: PTree.t nat) : res unit := OK tt. (* TODO *)
+Definition verify_mapping (f: function) (tc: code) (mp: PTree.t nat) : res unit := OK tt. (* TODO *)
 
 (** * Entry points *)
 
 Definition transf_function (f: function) : res function :=
-  let (tf, mp) := duplicate_aux f in
-  do u <- verify_mapping f tf mp;
-  OK tf.
+  let (tc, mp) := duplicate_aux f in
+  do u <- verify_mapping f tc mp;
+  OK (mkfunction (fn_sig f) (fn_params f) (fn_stacksize f) tc (fn_entrypoint f)).
+
+Theorem transf_function_preserves:
+  forall f tf,
+  transf_function f = OK tf ->
+     fn_sig f = fn_sig tf /\ fn_params f = fn_params tf /\ fn_stacksize f = fn_stacksize tf /\ fn_entrypoint f = fn_entrypoint tf.
+Proof.
+  intros. unfold transf_function in H. destruct (duplicate_aux _) as (tc & mp). monadInv H.
+  repeat (split; try reflexivity).
+Qed.
 
 Definition transf_fundef (f: fundef) : res fundef :=
   transf_partial_fundef transf_function f.
